src/storage.v
@@ -1,0 +1,43 @@
+(*===============================================================================
+    Model for the EVM storage or EVM execution environment
+   
+    Note that operations are partial, as not all storage is mapped.
+    Each storage cell is a EVMWORD - 256-bits.
+  ==============================================================================*)
+
+
+Require Import mathcomp.ssreflect.ssreflect.
+From mathcomp Require Import ssrfun ssrbool eqtype ssrnat seq fintype finfun.
+
+Require Import bitsrep bitsops cursor pmap reader writer.
+
+Set Implicit Arguments.
+Unset Strict Implicit.
+Import Prenex Implicits.
+
+(* 256-bit addressable storage of EVMWORD *)
+(*=Storage *)
+Definition Storage := PMAP EVMWORD 256.
+(*= End *)
+
+Definition PTR := EVMWORD.
+Identity Coercion PTRtoEVMWORD : PTR >-> EVMWORD.
+
+(* Initialize the storage, no cell is mapped *)
+Definition initialStorage : Storage := @EmptyPMap EVMWORD 256.
+
+(* Check the storage region from pointer [p] to just below pointer [p'] in [sto]
+   consists exactly the evmwords in [xs] *)
+Fixpoint stoIs (sto : Storage) (p p' : PTR) xs :=
+  if xs is x::xs then sto p = Some x /\ stoIs sto (incB p) p' xs
+  else p = p'.
+
+(* Map an evmword at [p] with 1-bits *)
+Definition reserveMemoryEVMWord (sto: Storage) (p : PTR) : Storage :=
+  sto !p := ones 256.
+
+(* Map storage region of [c] words at [p] with 1-bits *)
+Definition reserveStorage (sto : Storage) (p : PTR) (c : EVMWORD) : Storage :=
+  bIterFrom p c (fun p sto => sto !p := ones 256) sto.
+
+Definition isMappedStorage (p : PTR) (sto : Storage) : bool := sto p.
